First 2 step type redux

src/ReorderingRw.v
@@ -157,38 +157,18 @@ Definition rsrw_G_s_niff :=
     (exec_add_read_event_nctrl rsrw_G_s_iff a)
     (srf_s ⨾ ⦗eq a⦘).
 
-Lemma rsrw_struct_same_lab1
-    (INA : E_t a)
-    (INB : E_t b)
-    (STRUCT : reord_simrel_rw_struct) :
-  lab_s = (lab_t ∘ mapper).
-Proof using RSRW_ACTIDS.
-  rewrite rsrw_struct_same_lab; ins.
-  apply functional_extensionality. intro x.
-  tertium_non_datur (x = a) as [HEQ|NEQ]; subst; rupd; ins.
-  apply same_label_u2v_val.
-  { rewrite <- Combinators.compose_id_right with (f := lab_s),
-            <- ReordCommon.mapper_mapper_compose with (a := a) (b := b),
-            <- Combinators.compose_assoc; auto using rsrw_a_neq_b.
-    apply same_lab_u2v_compose; ins. apply STRUCT. }
-  rewrite STRUCT.(rsrw_lab_val_end); ins.
-  unfold val, compose. now rewrite ReordCommon.mapper_eq_a.
-Qed.
-
-Lemma rsrw_struct_same1
-    (INA : E_t a)
-    (INB : E_t b)
+Lemma rsrw_struct_iff
     (SAME : E_t a <-> E_t b) :
-  reord_simrel_rw_struct <->
-    exec_equiv G_s (exec_mapped G_t mapper (lab_t ∘ mapper)).
+  reord_simrel_rw_struct <-> exec_equiv G_s rsrw_G_s_iff.
 Proof using RSRW_ACTIDS.
   split; [intro STRUCT | intro EQUIV].
   { constructor; ins.
     all: try now apply STRUCT.
-    apply rsrw_struct_same_lab1; ins. }
+    admit. }
   assert (EQVLAB : lab_s = lab_t ∘ mapper).
-  { rewrite EQUIV.(exeeqv_lab _ _). ins. }
+  { admit. }
   constructor; ins.
+  all: try now (exfalso; desf; eauto).
   all: try now apply EQUIV.
   { rewrite EQVLAB. unfold val, compose.
     now rewrite ReordCommon.mapper_eq_a. }
@@ -202,79 +182,51 @@ Proof using RSRW_ACTIDS.
     now rewrite Combinators.compose_assoc, ReordCommon.mapper_mapper_compose,
             Combinators.compose_id_right by apply rsrw_a_neq_b. }
   now rewrite EQUIV.(exeeqv_acts _ _).
-Qed.
-
-Lemma rsrw_struct_same2
-    (INA : ~E_t a)
-    (INB : ~E_t b)
-    (SAME : E_t a <-> E_t b)
-    (U2V  : same_label_u2v (lab_s a) (lab_t b)) :
-  reord_simrel_rw_struct <->
-    exec_equiv G_s (exec_upd_lab
-      (exec_mapped G_t mapper (lab_t ∘ mapper))
-    a (lab_s a)).
-Proof using RSRW_ACTIDS.
-  split; [intro STRUCT | intro EQUIV].
-  { constructor; ins.
-    all: try now apply STRUCT.
-    apply rsrw_struct_same_lab; ins. }
-  assert (EQVLAB : lab_s = upd (lab_t ∘ mapper) a (lab_s a)).
-  { rewrite EQUIV.(exeeqv_lab _ _) at 1. ins. }
-  constructor; ins.
-  all: try now apply EQUIV.
-  { rewrite EQVLAB, upd_compose; [|apply ReordCommon.mapper_inj, rsrw_a_neq_b].
-    rewrite Combinators.compose_assoc, ReordCommon.mapper_mapper_compose,
-            Combinators.compose_id_right by apply rsrw_a_neq_b.
-    rewrite ReordCommon.mapper_eq_a. do 2 red. intros e _.
-    tertium_non_datur (e = b) as [HEQ|NEQ]; subst; rupd; ins.
-    red. desf. }
-  { rewrite EQVLAB, upd_compose; [|apply ReordCommon.mapper_inj, rsrw_a_neq_b].
-    rewrite ReordCommon.mapper_eq_a.
-    change (val (upd lab_t b (lab_s a) ∘ mapper) ∘ mapper)
-    with (val (upd lab_t b (lab_s a) ∘ mapper ∘ mapper)).
-    rewrite Combinators.compose_assoc, ReordCommon.mapper_mapper_compose,
-            Combinators.compose_id_right by apply rsrw_a_neq_b.
-    unfold val. rewrite updo; ins. }
-  rewrite EQUIV.(exeeqv_acts _ _); ins.
-Qed.
+Admitted.
 
 Lemma rsrw_struct_niff
     (INA : E_t a)
     (NOTINB : ~E_t b)
-    (U2V  : same_label_u2v (lab_s a) (lab_t b))
-    (EQVLAB : lab_s = upd (lab_t ∘ mapper) a (lab_s a)) :
-  reord_simrel_rw_struct <->
-    exec_equiv G_s (exec_add_rf
-      (exec_add_read_event_nctrl
-        (exec_upd_lab
-          (exec_mapped G_t mapper (lab_t ∘ mapper))
-          a (lab_s a)) a)
-      (srf_s ⨾ ⦗eq b⦘)).
+    (* (U2V  : same_label_u2v (lab_s a) (lab_t b))
+    (EQVLAB : lab_s = upd (lab_t ∘ mapper) a (lab_s a))  *)
+    :
+  reord_simrel_rw_struct <-> exec_equiv G_s rsrw_G_s_niff.
 Proof using RSRW_ACTIDS.
   split; [intro STRUCT | intro EQUIV].
   { constructor; ins.
-    all: try now apply STRUCT. }
+    all: try now apply STRUCT.
+    admit. }
   constructor; ins.
   all: try now apply EQUIV.
-  all: try now (exfalso; apply NOTINB, SAME, INA).
-  { rewrite EQVLAB, upd_compose; [| apply ReordCommon.mapper_inj, rsrw_a_neq_b].
-    rewrite Combinators.compose_assoc, ReordCommon.mapper_mapper_compose,
-            Combinators.compose_id_right by apply rsrw_a_neq_b.
-    rewrite ReordCommon.mapper_eq_a. do 2 red. intros e _.
-    tertium_non_datur (e = b) as [HEQ|NEQ]; subst; rupd; ins.
-    red. desf. }
-  { rewrite EQVLAB, upd_compose; [| apply ReordCommon.mapper_inj, rsrw_a_neq_b].
-    rewrite ReordCommon.mapper_eq_a.
-    change (val (upd lab_t b (lab_s a) ∘ mapper) ∘ mapper)
-      with (val (upd lab_t b (lab_s a)) ∘ mapper ∘ mapper).
-    rewrite Combinators.compose_assoc, ReordCommon.mapper_mapper_compose,
-            Combinators.compose_id_right by apply rsrw_a_neq_b.
-    unfold val. rupd. }
+  all: try now (exfalso; desf; eauto).
+  { admit. }
+  { admit. }
   rewrite EQUIV.(exeeqv_acts _ _); ins.
   rewrite set_inter_union_l.
   arewrite (eq a ∩₁ is_init ≡₁ ∅); [| now rewrite set_union_empty_r].
   split; [| basic_solver]. intros x (EQ & INIT). subst.
   red. now apply RSRW_ACTIDS.(rsrw_ninit_a).
+Admitted.
+
+Lemma rsrw_G_s_in_E e
+    (SIMREL : reord_simrel_rw)
+    (NOTA : e <> a)
+    (NOTB : e <> b) :
+  E_s e <-> E_t e.
+Proof using.
+  rewrite <- 2!set_subset_single_l with (a := e).
+  destruct (classic (E_t a)) as [INA|NINA],
+           (classic (E_t b)) as [INB|NINB].
+  { rewrite (rsrw_actids1 (rsrw_struct SIMREL)); ins.
+    rewrite ReordCommon.mapper_acts_iff; ins. }
+  { rewrite (rsrw_actids2 (rsrw_struct SIMREL)); ins.
+    rewrite ReordCommon.mapper_acts_niff; ins.
+    split; intros HSET; [| basic_solver].
+    unfolder in *. specialize HSET with e.
+    destruct HSET; ins; congruence. }
+  { exfalso. now apply (rsrw_actids_t_ord (rsrw_actids SIMREL)). }
+  rewrite (rsrw_actids1 (rsrw_struct SIMREL)); ins.
+  rewrite ReordCommon.mapper_acts_iff; ins.
 Qed.
 
 End SimRel.
@@ -319,11 +271,12 @@ Notation "'R_s'" := (is_r lab_s).
 Notation "'mapper'" := (ReordCommon.mapper a b).
 
 Lemma sim_rel_init
-    (ACTIDS : reord_simrel_rw_actids G_t a b)
+    (ACTIDS : reord_simrel_rw_actids G_s G_t a b)
     (STRUCT : reord_simrel_rw_struct G_s G_t a b) :
   reord_simrel_rw (WCore.init_exec G_s) (WCore.init_exec G_t) a b.
 Proof using.
-  constructor; constructor; ins.
+  admit.
+  (* constructor; constructor; ins.
   all: try now (rewrite collect_rel_empty; ins).
   all: try now (exfalso; apply ACTIDS.(rsrw_ninit_a G_t a b), INA).
   all: try now apply ACTIDS.
@@ -332,14 +285,15 @@ Proof using.
   all: rewrite STRUCT.(rsrw_init _ _ _ _).
   all: rewrite set_collect_interE, ReordCommon.mapper_is_init; ins.
   all: try now apply ACTIDS.
-  all: eapply ReordCommon.mapper_inj, rsrw_a_neq_b; eauto.
-Qed.
+  all: eapply ReordCommon.mapper_inj, rsrw_a_neq_b; eauto. *)
+Admitted.
 
 End Basic.
 
 Section SimrelExec.
 
 Variable G_t G_t' G_s : execution.
+Variable sc : relation actid.
 Variable traces traces' : thread_id -> trace label -> Prop.
 Variable a b : actid.
 
@@ -393,850 +347,290 @@ Notation "'srf_s'" := (srf G_s).
 Notation "'mapper'" := (ReordCommon.mapper a b).
 
 Hypothesis SWAPPED_TRACES : ReordCommon.traces_swapped traces traces' a b.
+Hypothesis SIMREL : reord_simrel_rw G_s G_t a b.
 
-(*
-  Big case 1: both events are in the target execution.
+Definition G_s' :=
+  ifP E_t' a /\ ~E_t' b then rsrw_G_s_niff G_s G_t' a b
+  else rsrw_G_s_iff G_s G_t' a b.
 
-  At this point out labeling function must match up with
-  the target execution.
-*)
-Lemma simrel_exec_iff_helper_1 sc e
-    (SAME : E_t a <-> E_t b)
+Notation "'lab_s''" := (lab G_s').
+Notation "'val_s''" := (val lab_s').
+Notation "'E_s''" := (acts_set G_s').
+Notation "'loc_s''" := (loc lab_s').
+Notation "'sb_s''" := (sb G_s').
+Notation "'rf_s''" := (rf G_s').
+Notation "'co_s''" := (co G_s').
+Notation "'rmw_s''" := (rmw G_s').
+Notation "'rpo_s''" := (rpo G_s').
+Notation "'rmw_dep_s''" := (rmw_dep G_s').
+Notation "'data_s''" := (data G_s').
+Notation "'ctrl_s''" := (ctrl G_s').
+Notation "'addr_s''" := (addr G_s').
+Notation "'W_s''" := (is_w lab_s').
+Notation "'R_s''" := (is_r lab_s').
+Notation "'srf_s''" := (srf G_s').
+
+Lemma G_s_niff
     (INA : E_t a)
-    (INB : E_t b)
-    (E_NOT_A : e <> a)
-    (E_NOT_B : e <> b)
-    (CONS : WCore.is_cons G_t sc)
-    (STEP : WCore.exec_inst G_t G_t' sc traces e)
-    (SIM_ACTS : reord_simrel_rw_actids G_t a b)
-    (NRMWDEP : ~rmw_dep_t' a b)
-    (NRMW : ~rmw_t' a b)
-    (NRMWCODOM : ~codom_rel rmw_t' a)
-    (NRMWDOM : ~dom_rel rmw_t' b) :
-  WCore.exec_inst
-    (exec_mapped G_t  mapper (lab_t'  ∘ mapper))
-    (exec_mapped G_t' mapper (lab_t'  ∘ mapper))
-    (mapper ↑ sc)
-    traces'
-    e.
-Proof using.
-  (* Useful props *)
-  assert (NEQ : a <> b).
-  { intro F; eapply ext_sb_irr with (x := a).
-    rewrite F at 2. apply SIM_ACTS. }
-  assert (FIN_LAB : lab G_t' = lab_t).
-  { symmetry. eapply sub_lab.
-    eapply WCore.wf_g_sub_gc
-    with (X := {|
-      WCore.G := G_t;
-      WCore.GC := G_t';
-      WCore.sc := sc;
-      WCore.cmt := ∅;
-    |}).
-    apply STEP. }
-  assert (LABEQ : lab_t = lab_t ∘ mapper ∘ mapper).
-  { now rewrite Combinators.compose_assoc,
-                ReordCommon.mapper_mapper_compose,
-                Combinators.compose_id_right. }
-  assert (SAME' : E_t' a <-> E_t' b).
-  { destruct STEP. split; intro HSET.
-    all: apply (WCore.cae_e_new add_event).
-    all: apply (WCore.cae_e_new add_event) in HSET.
-    all: ins; unfolder; unfolder in HSET; desf.
-    all: now left. }
+    (NINB : ~E_t b) :
+  G_s = rsrw_G_s_niff G_s G_t a b.
+Proof using SIMREL.
+  apply exeeqv_eq, rsrw_struct_niff; eauto.
+  all: apply SIMREL.
+Qed.
 
-  (* actual proof *)
-  constructor; ins.
-  { replace ∅ with (mapper ↑₁ ∅) by now rewrite set_collect_empty.
-    admit. }
-  { destruct STEP. red in add_event. desf.
-    exists (option_map mapper r), (option_map mapper w),
-           (mapper ↑₁ W1), (mapper ↑₁ W2).
-    splits; ins.
-    { admit. }
-    { replace ∅ with (mapper ↑₁ ∅) by now rewrite set_collect_empty.
-      replace e with (mapper e) by now rewrite ReordCommon.mapper_neq.
-      apply cfg_mapped_add_step_props with
-        (X := {|
-            WCore.sc := sc;
-            WCore.G := G_t;
-            WCore.GC := G_t';
-            WCore.cmt := ∅;
-        |})
-        (X' := {|
-            WCore.sc := sc;
-            WCore.G := G_t';
-            WCore.GC := G_t';
-            WCore.cmt := ∅;
-        |}).
-      { now apply ReordCommon.mapper_inj. }
-      { now apply ReordCommon.mapper_surj. }
-      { ins. now rewrite FIN_LAB. }
-      apply PROPS. }
-    { admit. (* TODO: traces *) }
-    replace ∅ with (mapper ↑₁ ∅) by now rewrite set_collect_empty.
-    admit. }
-  admit. (* TODO: research *)
+Lemma G_s_iff
+    (INA : E_t a <-> E_t b) :
+  G_s = rsrw_G_s_iff G_s G_t a b.
+Proof using SIMREL.
+  apply exeeqv_eq, rsrw_struct_iff; eauto.
+  all: apply SIMREL.
+Qed.
+
+Lemma srf_eq
+    (INA : E_t a) :
+  exists sw,
+    srf_s ⨾ ⦗eq a⦘ = singl_rel sw a.
+Proof using.
+  admit.
 Admitted.
 
-(*
-  Big case 2: neither events are in the target graph.
+Definition X_t := {|
+  WCore.G := G_t;
+  WCore.GC := G_t';
+  WCore.sc := sc;
+  WCore.cmt := ∅;
+|}.
+Definition X_t' := {|
+  WCore.G := G_t';
+  WCore.GC := G_t';
+  WCore.sc := sc;
+  WCore.cmt := ∅;
+|}.
 
-  This means our labeling function must match target' almost
-  1-to-1, allowing some liberties with b's label. This condition
-  must be satisfied even right now, because we do not update our
-  labeling function during simple instruction steps.
-*)
-Lemma simrel_exec_iff_helper_2 sc e l
-    (U2V : same_label_u2v (lab_t' b) l)
-    (SAME : E_t a <-> E_t b)
-    (NINA : ~E_t a)
-    (NINB : ~E_t b)
+Definition rsrw_X_s_iff := cfg_upd_lab
+  (cfg_mapped X_t mapper (lab_t ∘ mapper))
+  a (lab_s a).
+Definition rsrw_X_s_niff := cfg_add_read_event_nctrl
+  rsrw_X_s_iff a (srf_s ⨾ ⦗eq a⦘).
+Definition rsrw_X_s'_iff := cfg_upd_lab
+  (cfg_mapped X_t' mapper (lab_t ∘ mapper))
+  a (lab_s a).
+Definition rsrw_X_s'_niff := cfg_add_read_event_nctrl
+  rsrw_X_s'_iff a (srf_s ⨾ ⦗eq a⦘).
+
+Lemma G_t_labs
+    (WF : WCore.wf X_t) :
+  lab_t' = lab_t.
+Proof using.
+  symmetry. apply WF.
+Qed.
+
+Lemma rsrw_X_s_iff_eq
+  (WF : WCore.wf X_t) :
+    {|
+      WCore.sc := mapper ↑ sc;
+      WCore.G := rsrw_G_s_iff G_s G_t a b;
+      WCore.GC := rsrw_G_s_iff G_s G_t' a b;
+      WCore.cmt := ∅
+    |} = rsrw_X_s_iff.
+Proof using.
+  unfold rsrw_X_s_iff, cfg_upd_lab, cfg_mapped,
+         cfg_add_read_event_nctrl,
+         rsrw_G_s_iff, X_t.
+  ins. f_equal; ins.
+  { now rewrite G_t_labs. }
+  apply set_extensionality. basic_solver.
+Qed.
+
+Lemma rsrw_X_s_niff_eq
+  (WF : WCore.wf X_t) :
+    {|
+      WCore.sc := mapper ↑ sc;
+      WCore.G := rsrw_G_s_niff G_s G_t a b;
+      WCore.GC := rsrw_G_s_niff G_s G_t' a b;
+      WCore.cmt := ∅
+    |} = rsrw_X_s_niff.
+Proof using.
+  unfold rsrw_X_s_niff.
+  rewrite <- rsrw_X_s_iff_eq; ins.
+Qed.
+
+Lemma rsrw_X_s'_iff_eq
+  (WF : WCore.wf X_t) :
+    {|
+      WCore.sc := mapper ↑ sc;
+      WCore.G := rsrw_G_s_iff G_s G_t' a b;
+      WCore.GC := rsrw_G_s_iff G_s G_t' a b;
+      WCore.cmt := ∅
+    |} = rsrw_X_s'_iff.
+Proof using.
+  unfold rsrw_X_s'_iff, cfg_upd_lab, cfg_mapped,
+         cfg_add_read_event_nctrl,
+         rsrw_G_s_iff, X_t.
+  ins. f_equal; ins.
+  all: try now rewrite G_t_labs.
+  apply set_extensionality. basic_solver.
+Qed.
+
+Lemma rsrw_X_s'_niff_eq
+  (WF : WCore.wf X_t) :
+    {|
+      WCore.sc := mapper ↑ sc;
+      WCore.G := rsrw_G_s_niff G_s G_t' a b;
+      WCore.GC := rsrw_G_s_niff G_s G_t' a b;
+      WCore.cmt := ∅
+    |} = rsrw_X_s'_niff.
+Proof using.
+  unfold rsrw_X_s'_niff.
+  rewrite <- rsrw_X_s'_iff_eq; ins.
+Qed.
+
+Lemma simrel_exec_not_a_not_b e
     (E_NOT_A : e <> a)
     (E_NOT_B : e <> b)
     (CONS : WCore.is_cons G_t sc)
-    (STEP : WCore.exec_inst G_t G_t' sc traces e)
-    (SIM_ACTS : reord_simrel_rw_actids G_t a b)
-    (NRMWDEP : ~rmw_dep_t' a b)
-    (NRMW : ~rmw_t' a b)
-    (NRMWCODOM : ~codom_rel rmw_t' a)
-    (NRMWDOM : ~dom_rel rmw_t' b) :
-  WCore.exec_inst
-    (exec_upd_lab
-      (exec_mapped G_t  mapper (lab_t'  ∘ mapper))
-      a l)
-    (exec_upd_lab
-      (exec_mapped G_t' mapper (lab_t' ∘ mapper))
-      a l)
-    (mapper ↑ sc)
-    traces'
-    e.
-Proof using.
-  (* Helper asserts *)
-  assert (NEQ : a <> b).
-  { intro F; eapply ext_sb_irr with (x := a).
-    rewrite F at 2. apply SIM_ACTS. }
-  assert (FIN_LAB : lab G_t' = lab_t).
-  { symmetry. eapply sub_lab.
-    eapply WCore.wf_g_sub_gc
-    with (X := {|
-      WCore.G := G_t;
-      WCore.GC := G_t';
-      WCore.sc := sc;
-      WCore.cmt := ∅;
-    |}).
-    apply STEP. }
-  assert (LABEQ : lab_t = lab_t ∘ mapper ∘ mapper).
-  { now rewrite Combinators.compose_assoc,
-                ReordCommon.mapper_mapper_compose,
-                Combinators.compose_id_right. }
-  assert (LABEQ' : upd lab_t b l = upd (lab_t ∘ mapper) a l ∘ mapper).
-  { ins; unfold compose.
-    apply functional_extensionality; intro x.
-    tertium_non_datur (x = b) as [HEQ|HEQ]; subst.
-    { now rewrite ReordCommon.mapper_eq_b, !upds. }
-    rewrite !updo, ReordCommon.mapper_self_inv; ins.
-    intro F; rewrite <- ReordCommon.mapper_eq_b with (b := b) in F.
-    apply ReordCommon.mapper_inj in F; ins. }
-  assert (NINA' : ~E_t' a).
-  { intro F'. destruct STEP; ins.
-    apply (WCore.cae_e_new add_event) in F'.
-    ins. destruct F' as [HIN|HEQ]; desf. }
-  assert (NINB' : ~E_t' b).
-  { intro F'. destruct STEP; ins.
-    apply (WCore.cae_e_new add_event) in F'.
-    ins. destruct F' as [HIN|HEQ]; desf. }
-  assert (ANREAD : ~ codom_rel (mapper ↑ rf_t') a).
-  { unfolder. intro F. desf.
-    rewrite ReordCommon.mapper_inj with (a := a) (b := b)
-                                        (x := y') (y := b) in F.
-    all: ins; try now rewrite ReordCommon.mapper_eq_b.
-    apply NINB'.
-    apply (wf_rfE (WCore.wf_gc (WCore.start_wf STEP))) in F.
-    ins. unfolder in F. desf. }
-  assert (BNREAD : ~ dom_rel (mapper ↑ rf_t') a).
-  { unfolder. intro F. desf.
-    rewrite ReordCommon.mapper_inj with (a := a) (b := b)
-                                        (x := x') (y := b) in F.
-    all: ins; try now rewrite ReordCommon.mapper_eq_b.
-    apply NINB'.
-    apply (wf_rfE (WCore.wf_gc (WCore.start_wf STEP))) in F.
-    ins. unfolder in F. desf. }
-  assert (ACTEQ : E_t' ≡₁ E_t ∪₁ eq e).
-  { destruct STEP.
-    rewrite (WCore.cae_e_new add_event). ins. }
+    (STEP : WCore.exec_inst G_t G_t' sc traces e) :
+  exists G_s' sc',
+    << SIMREL : reord_simrel_rw G_s' G_t' a b >> /\
+    << STEP : WCore.exec_inst G_s G_s' sc' traces' e >>.
+Proof using SIMREL.
+  (* Preamble *)
+  destruct STEP as [STARTWF ADD]. red in ADD. desf.
+  assert (INAIFF : E_t a <-> E_t' a).
+  { rewrite <- 2!set_subset_single_l with (a := a).
+    rewrite (WCore.caes_e_new STRUCT); ins.
+    rewrite 2!set_subset_single_l.
+    unfolder; split; ins; desf; eauto. }
+  assert (INBIFF : E_t b <-> E_t' b).
+  { rewrite <- 2!set_subset_single_l with (a := b).
+    rewrite (WCore.caes_e_new STRUCT); ins.
+    rewrite 2!set_subset_single_l.
+    unfolder; split; ins; desf; eauto. }
+  assert (IFFSHORTCUT : forall (CASE2 : ~ (E_t' a /\ ~E_t' b)),
+                        E_t a <-> E_t b).
+  { desf.
+    destruct (classic (E_t a)) as [INA|NINA],
+             (classic (E_t b)) as [INB|NINB]; ins.
+    { exfalso. eauto 11. }
+    exfalso. apply (rsrw_actids_t_ord (rsrw_actids SIMREL)).
+    all: ins. }
+  assert (IFFSHORTCUT' : forall (CASE2 : ~ (E_t' a /\ ~E_t' b)),
+                        E_t' a <-> E_t' b).
+  { ins. rewrite <- INAIFF, <- INBIFF. eauto. }
   (* Actual proof *)
-  destruct STEP; ins. red in add_event. desf.
-  constructor; ins.
-  { replace ∅ with (mapper ↑₁ ∅); [| now rewrite set_collect_empty].
-    apply cfg_upd_lab_wf with (X := {|
-      WCore.sc := mapper ↑ sc;
-      WCore.G := exec_mapped G_t mapper (lab_t' ∘ mapper);
-      WCore.GC := exec_mapped G_t' mapper (lab_t' ∘ mapper);
-      WCore.cmt := mapper ↑₁ ∅
-    |}); ins.
-    { apply SIM_ACTS. }
-    { unfold compose. now rewrite ReordCommon.mapper_eq_a. }
-    admit. }
+  exists G_s', (mapper ↑ sc). split; constructor; ins.
+  { admit. (* TODO: simrel actids *) }
+  { admit. (* TODO: simrel struct *) }
+  { admit. (* TODO: simrel start wf *) }
   { exists (option_map mapper r), (option_map mapper w),
            (mapper ↑₁ W1), (mapper ↑₁ W2).
     splits.
     { constructor; ins.
-      { rewrite ACTEQ, set_collect_union, set_collect_eq,
-                ReordCommon.mapper_neq; ins. }
-      { unfolder. intro F. desf.
-        apply STRUCT. ins.
-        rewrite ReordCommon.mapper_neq; ins.
-        { intro EQ; subst. apply E_NOT_B.
-          now rewrite ReordCommon.mapper_eq_a. }
-        intro EQ; subst. apply E_NOT_A.
-        now rewrite ReordCommon.mapper_eq_b. }
+      { unfold G_s'. desf; ins.
+        { desf. rewrite G_s_niff; ins; eauto.
+          rewrite !ReordCommon.mapper_acts_niff; eauto.
+          rewrite (WCore.caes_e_new STRUCT); ins.
+          basic_solver. }
+        rewrite G_s_iff; ins; eauto.
+        rewrite !ReordCommon.mapper_acts_iff; eauto.
+        now rewrite (WCore.caes_e_new STRUCT). }
+      { rewrite rsrw_G_s_in_E with (a := a) (b := b); eauto.
+        apply STRUCT. }
       apply STRUCT. }
-    { replace ∅ with (mapper ↑₁ ∅) by now rewrite set_collect_empty.
+    { unfold G_s'. desf.
+      { desf. rewrite G_s_niff at 1; ins; eauto.
+        destruct srf_eq as (sw & SRFEQ); eauto.
+        replace e with (mapper e) by now rewrite ReordCommon.mapper_neq.
+        rewrite rsrw_X_s'_niff_eq, rsrw_X_s_niff_eq; ins.
+        unfold rsrw_X_s_niff, rsrw_X_s'_niff. rewrite SRFEQ.
+        apply cfg_add_event_nctrl_add_step_props.
+        { ins. admit. }
+        apply cfg_upd_lab_add_step_props.
+        { ins. admit. }
+        eapply cfg_mapped_add_step_props; ins.
+        all: admit. }
+      desf. rewrite G_s_iff at 1; ins; eauto.
       replace e with (mapper e) by now rewrite ReordCommon.mapper_neq.
-      apply cfg_upd_lab_add_step_props with
-        (X := {|
-          WCore.sc := mapper ↑ sc;
-          WCore.G := exec_mapped G_t  _ _;
-          WCore.GC := exec_mapped G_t' _ _;
-          WCore.cmt := mapper ↑₁ ∅
-        |})
-        (X' := {|
-          WCore.sc := mapper ↑ sc;
-          WCore.G := exec_mapped G_t'  _ _;
-          WCore.GC := exec_mapped G_t' _ _;
-          WCore.cmt := mapper ↑₁ ∅
-        |}).
-      { ins. unfold compose. now rewrite ReordCommon.mapper_eq_a. }
-      apply cfg_mapped_add_step_props with
-        (X := {|
-            WCore.sc := sc;
-            WCore.G := G_t;
-            WCore.GC := G_t';
-            WCore.cmt := ∅;
-        |})
-        (X' := {|
-            WCore.sc := sc;
-            WCore.G := G_t';
-            WCore.GC := G_t';
-            WCore.cmt := ∅;
-        |}).
-      { now apply ReordCommon.mapper_inj. }
-      { now apply ReordCommon.mapper_surj. }
-      { ins. now rewrite FIN_LAB. }
-      apply PROPS. }
-    { admit. (* traces *) }
-    replace ∅ with (mapper ↑₁ ∅); [| now rewrite set_collect_empty].
-    apply cfg_upd_lab_wf with (X := {|
-      WCore.sc := mapper ↑ sc;
-      WCore.G := exec_mapped G_t' mapper (lab_t' ∘ mapper);
-      WCore.GC := exec_mapped G_t' mapper (lab_t' ∘ mapper);
-      WCore.cmt := mapper ↑₁ ∅;
-    |}); ins.
-    { apply SIM_ACTS. }
-    { unfold compose. now rewrite ReordCommon.mapper_eq_a. }
-    admit. }
-  admit. (* TODO: Is_cons *)
-Admitted.
-
-Lemma simrel_exec_niff_helper sc e l sw
-    (U2V : same_label_u2v (lab_t' b) l)
-    (E_NOT_A : e <> a)
-    (E_NOT_B : e <> b)
-    (W_NOT_A : sw <> a)
-    (W_NOT_B : sw <> b)
-    (B_TID : tid a <> tid_init)
-    (CONS : WCore.is_cons G_t sc)
-    (STEP : WCore.exec_inst G_t G_t' sc traces e)
-    (SIM_ACTS : reord_simrel_rw_actids G_t a b)
-    (WB_LOC : same_loc (upd (lab_t' ∘ mapper) a l) a sw)
-    (WB_VAL : val (upd (lab_t' ∘ mapper) a l) sw =
-              val (upd (lab_t' ∘ mapper) a l) a)
-    (HWIN : E_t sw)
-    (W_IS : W_t sw)
-    (INA :   E_t a)
-    (NINB : ~E_t b)
-    (BINIT : forall l0 (LOC : loc lab_t' b = Some l0), E_t' (InitEvent l0))
-    (NRMWDEP : ~rmw_dep_t' a b)
-    (NRMW : ~rmw_t' a b)
-    (NRMWCODOM : ~codom_rel rmw_t' a)
-    (NRMWDOM : ~dom_rel rmw_t' b) :
-  WCore.exec_inst
-    (exec_add_rf
-      (exec_add_read_event_nctrl
-        (exec_upd_lab
-          (exec_mapped G_t mapper (lab_t' ∘ mapper))
-          a l) a)
-      (singl_rel sw a))
-    (exec_add_rf
-      (exec_add_read_event_nctrl
-        (exec_upd_lab
-          (exec_mapped G_t' mapper (lab_t' ∘ mapper))
-          a l) a)
-      (singl_rel sw a))
-    (mapper ↑ sc)
-    traces'
-    e.
-Proof using.
-  assert (ANEQB : a <> b).
-  { eapply rsrw_a_neq_b; eauto. }
-  assert (INA' : E_t' a).
-  { destruct STEP; ins.
-    apply (WCore.cae_e_new add_event).
-    ins. now left. }
-  assert (NINB' : ~E_t' b).
-  { intro F'. destruct STEP; ins.
-    apply (WCore.cae_e_new add_event) in F'.
-    ins. destruct F' as [HIN|HEQ]; desf. }
-  assert (FIN_LAB : lab G_t' = lab_t).
-  { symmetry. destruct STEP; ins.
-    now apply WCore.wf_g_sub_gc
-    with (X := {|
-      WCore.G := G_t;
-      WCore.GC := G_t';
-      WCore.sc := sc;
-      WCore.cmt := ∅;
-    |}). }
-  assert (LABEQ : lab_t' = lab_t' ∘ mapper ∘ mapper).
-  { rewrite Combinators.compose_assoc.
-    rewrite ReordCommon.mapper_mapper_compose; eauto. }
-  assert (IS_W_SAME : is_w (upd (lab_t' ∘ mapper) a l) e = W_t' e).
-  { unfold compose, is_w.
-    now rewrite updo, ReordCommon.mapper_neq. }
-  assert (A_NMAPPED : ~ (mapper ↑₁ E_t') a).
-  { unfolder. intro F. desf.
-    apply NINB'. arewrite (b = y); ins.
-    apply ReordCommon.mapper_inj with (a := a) (b := b); ins.
-    now rewrite ReordCommon.mapper_eq_b. }
-  assert (A_IS_R : is_r (upd (lab_t' ∘ mapper) a l) a).
-  { unfold is_r, compose. rewrite upds.
-    red in U2V. desf; exfalso.
-    all: enough (BNOTR : ~R_t b) by apply BNOTR, SIM_ACTS.
-    all: now unfold is_r; rewrite <- FIN_LAB, Heq. }
-  (* Actual proof *)
-  constructor; ins.
-  { replace ∅ with (mapper ↑₁ ∅); [| now rewrite set_collect_empty].
-    apply WCore.wf_iff_struct_and_props; split.
-    { destruct STEP. constructor; ins.
-      { unfold FinThreads.fin_threads. ins.
-        apply start_wf. }
-      { now rewrite (WCore.wf_cc_ctrl_empty start_wf), collect_rel_empty. }
-      { now rewrite (WCore.wf_cc_addr_empty start_wf), collect_rel_empty. }
-      { now rewrite (WCore.wf_cc_data_empty start_wf), collect_rel_empty. }
-      { apply exec_add_rf_cont. admit. (* TODO: need weaker lemma *) }
-      { apply exec_add_rf_cont. admit. }
-      { intros x [[INE | EQA] HINIT]; try now right.
-        destruct INE as (x' & INE & HEQ).
-        left. exists x'; split; eauto.
-        apply (WCore.wf_g_init start_wf); split; ins.
-        erewrite ReordCommon.mapper_inj with (x := x') (y := x)
-                                             (a := a) (b := b).
-        all: ins.
-        destruct x as [xl | xtid xid]; ins.
-        rewrite ReordCommon.mapper_init_actid with (a := a) (b := b).
-        all: ins; now apply SIM_ACTS. }
-      intros x [EQTID [INE | EQA]]; red in EQTID.
-      { apply (WCore.wf_gc_acts start_wf); split; ins.
-        destruct INE as (x' & INE & HEQ).
-        rewrite ReordCommon.mapper_neq in HEQ; subst; ins.
-        all: intro F'; subst x'; eauto.
-        apply B_TID. erewrite rsrw_tid_a_tid_b; eauto.
-        rewrite ReordCommon.mapper_eq_a; eauto. }
-      subst; exfalso; apply SIM_ACTS.(rsrw_ninit_a _ _ _).
-      apply (WCore.wf_gc_acts start_wf); split; ins. }
-    apply cfg_add_event_nctrl_wf_props with (X := {|
-      WCore.sc := mapper ↑ sc;
-      WCore.G := exec_upd_lab _ a l;
-      WCore.GC := exec_upd_lab _ a l;
-      WCore.cmt := mapper ↑₁ ∅
-    |}); ins.
-    { apply SIM_ACTS. }
-    { apply STEP. ins. }
-    { admit. (* TODO: a is sb-max *) }
-    { unfolder. exists (InitEvent l0).
-      split; [| apply ReordCommon.mapper_init_actid].
-      all: try now apply SIM_ACTS.
-      apply BINIT. unfold loc in *.
-      rewrite upds in LOC. red in U2V.
-      do 2 desf. }
-    { unfolder in DOM2. desf.
-      unfolder in DOM1. desf.
-      apply NINB'.
-      rewrite ReordCommon.mapper_inj with (x := b) (y := y')
-                                          (a := a) (b := b).
-      all: ins; try now rewrite ReordCommon.mapper_eq_b.
-      destruct STEP.
-      apply (wf_rfE (WCore.wf_gc start_wf)) in DOM1.
-      ins. unfolder in DOM1; desf. }
-    { unfolder. ins. desf. }
-    { unfolder. ins. desf. }
-    { unfolder. splits; ins; desf.
-      splits; eauto. left.
-      exists sw. split; ins.
-      rewrite ReordCommon.mapper_neq; ins. }
-    { unfolder. splits; ins; desf.
-      splits; eauto; unfold is_w, is_r, compose; rupd.
-      rewrite ReordCommon.mapper_neq; ins. now rewrite FIN_LAB. }
-    { unfolder. ins. desf. }
-    { unfolder. eauto. }
-    { admit. }
-    { admit. }
-    apply cfg_upd_lab_wf_props with (e := a) (l := l) (X := {|
-      WCore.sc := mapper ↑ sc;
-      WCore.G := exec_mapped G_t mapper (lab_t' ∘ mapper);
-      WCore.GC := exec_mapped G_t' mapper (lab_t' ∘ mapper);
-      WCore.cmt := mapper ↑₁ ∅;
-    |}); ins.
-    { apply SIM_ACTS. }
-    { unfold compose. now rewrite ReordCommon.mapper_eq_a. }
-    { unfolder. intro F. desf.
-      apply (wf_rfE (WCore.wf_gc (WCore.start_wf STEP))) in F.
-      ins. unfolder in F. desf.
-      apply NINB'.
-      rewrite ReordCommon.mapper_inj with (a := a) (b := b)
-                                          (x := b) (y := y').
-      all: ins.
-      now rewrite ReordCommon.mapper_eq_b. }
-    { unfolder. intro F. desf.
-      apply (wf_rfE (WCore.wf_gc (WCore.start_wf STEP))) in F.
-      ins. unfolder in F. desf.
-      apply NINB'.
-      rewrite ReordCommon.mapper_inj with (a := a) (b := b)
-                                          (x := b) (y := x').
-      all: ins.
-      now rewrite ReordCommon.mapper_eq_b. }
-    apply cfg_mapped_wf_props with (X := {|
-      WCore.sc := sc;
-      WCore.G := G_t;
-      WCore.GC := G_t';
-      WCore.cmt := ∅;
-    |}); ins.
-    all: try now apply STEP.
-    { apply ReordCommon.mapper_inj. eapply rsrw_a_neq_b; eauto. }
-    { admit. }
-    { apply ReordCommon.mapper_init_actid. apply SIM_ACTS.(rsrw_ninit_a G_t a b).
-      apply SIM_ACTS.(rsrw_ninit_b G_t a b). }
-    { apply ReordCommon.mapped_G_t_immsb_helper; ins.
-      all: try now apply SIM_ACTS.
-      apply STEP. }
-    { apply ReordCommon.mapped_G_t_sb_helper; ins.
-      all: try now apply SIM_ACTS.
-      apply STEP. }
-    (* FIXME: uses auto gen names *)
-    { admit. (* TODO: lemma *) }
-    admit. }
-  { replace ∅ with (mapper ↑₁ ∅) by now rewrite set_collect_empty.
-    replace e with (mapper e) by now rewrite ReordCommon.mapper_neq.
-    destruct STEP. red in add_event. desf. ins.
-    exists (option_map mapper r), (option_map mapper w),
-           (mapper ↑₁ W1), (mapper ↑₁ W2).
-    splits.
-    { admit. }
-    { apply cfg_add_event_nctrl_add_step_props with
-        (X := {|
-          WCore.sc := mapper ↑ sc;
-          WCore.G := exec_mapped G_t  _ _;
-          WCore.GC := exec_mapped G_t' _ _;
-          WCore.cmt := mapper ↑₁ ∅
-        |})
-        (X' := {|
-          WCore.sc := mapper ↑ sc;
-          WCore.G := exec_mapped G_t'  _ _;
-          WCore.GC := exec_mapped G_t' _ _;
-          WCore.cmt := mapper ↑₁ ∅
-        |}).
-      { ins. intro F. apply set_collect_empty in F.
-        desf. }
-      apply cfg_upd_lab_add_step_props with
-        (X := {|
-          WCore.sc := mapper ↑ sc;
-          WCore.G := exec_mapped G_t  _ _;
-          WCore.GC := exec_mapped G_t' _ _;
-          WCore.cmt := mapper ↑₁ ∅
-        |})
-        (X' := {|
-          WCore.sc := mapper ↑ sc;
-          WCore.G := exec_mapped G_t'  _ _;
-          WCore.GC := exec_mapped G_t' _ _;
-          WCore.cmt := mapper ↑₁ ∅
-        |}).
-      { ins. unfold compose. now rewrite ReordCommon.mapper_eq_a. }
-      apply cfg_mapped_add_step_props with
-        (X := {|
-            WCore.sc := sc;
-            WCore.G := G_t;
-            WCore.GC := G_t';
-            WCore.cmt := ∅;
-        |})
-        (X' := {|
-            WCore.sc := sc;
-            WCore.G := G_t';
-            WCore.GC := G_t';
-            WCore.cmt := ∅;
-        |}).
-      { now apply ReordCommon.mapper_inj. }
-      { now apply ReordCommon.mapper_surj. }
-      { ins. }
-      apply PROPS. }
-    { admit. (* Trace *) }
-    apply WCore.wf_iff_struct_and_props; split.
-    { constructor; ins.
-      { unfold FinThreads.fin_threads. ins.
-        apply start_wf. }
-      { now rewrite (WCore.wf_cc_ctrl_empty start_wf), collect_rel_empty. }
-      { now rewrite (WCore.wf_cc_addr_empty start_wf), collect_rel_empty. }
-      { now rewrite (WCore.wf_cc_data_empty start_wf), collect_rel_empty. }
-      { apply exec_add_rf_cont. admit. (* TODO: need weaker lemma *) }
-      { apply exec_add_rf_cont. admit. }
-      { intros x [[INE | EQA] HINIT]; try now right.
-        destruct INE as (x' & INE & HEQ).
-        left. exists x'; split; eauto. }
-      intros x [EQTID [INE | EQA]]; red in EQTID.
-      { apply (WCore.wf_gc_acts start_wf); split; ins.
-        destruct INE as (x' & INE & HEQ).
-        rewrite ReordCommon.mapper_neq in HEQ; subst; ins.
-        all: intro F'; subst x'; eauto.
-        apply B_TID. erewrite rsrw_tid_a_tid_b; eauto.
-        rewrite ReordCommon.mapper_eq_a; eauto. }
-      subst; exfalso; apply SIM_ACTS.(rsrw_ninit_a _ _ _).
-      apply (WCore.wf_gc_acts start_wf); split; ins. }
-    apply cfg_add_event_nctrl_wf_props with (X := {|
-      WCore.sc := mapper ↑ sc;
-      WCore.G := exec_upd_lab _ a l;
-      WCore.GC := exec_upd_lab _ a l;
-       WCore.cmt := mapper ↑₁ ∅
-    |}); ins.
-    { apply SIM_ACTS. }
-    { apply start_wf. ins. }
-    { admit. }
-    { admit. }
-    { admit. }
-    { unfolder. ins. desf. }
-    { unfolder. ins. desf. }
-    { admit. }
-    { admit. }
-    { unfolder. ins. desf. }
-    { unfolder. eauto. }
-    { admit. }
-    { admit. }
-    apply cfg_upd_lab_wf_props with (X := {|
-      WCore.sc := mapper ↑ sc;
-      WCore.G := exec_mapped _ _ _;
-      WCore.GC := exec_mapped _ _ _;
-      WCore.cmt := mapper ↑₁ ∅;
-    |}); ins.
-    all: admit. }
+      rewrite rsrw_X_s'_iff_eq, rsrw_X_s_iff_eq; ins.
+      unfold rsrw_X_s_iff, rsrw_X_s'_iff.
+      apply cfg_upd_lab_add_step_props.
+      { ins. admit. }
+      eapply cfg_mapped_add_step_props; ins.
+      all: admit. }
+    { admit. (* TODO: traces *) }
+    admit. (* TODO: end wf *) }
   admit.
 Admitted.
 
-(*
-  Lemma that unites to big cases into one megacase: iff.
-
-  This is when both events are either present or absent in the
-  target execution.
-*)
-Lemma simrel_exec_iff e sc
-    (SAME : E_t a <-> E_t b)
-    (E_NOT_A : e <> a)
-    (E_NOT_B : e <> b)
+Lemma simrel_exec_b_helper
     (CONS : WCore.is_cons G_t sc)
-    (STEP : WCore.exec_inst G_t G_t' sc traces e)
-    (SIM : reord_simrel_rw G_s G_t a b) :
-  exists G_s' sc',
-    WCore.exec_inst G_s G_s' sc' traces' e.
-Proof using.
-  assert (NRMWDEP : ~rmw_dep_t' a b).
-  { admit. }
-  assert (NRMW : ~rmw_t' a b).
-  { admit. }
-  assert (NRMWCODOM : ~codom_rel rmw_t' a).
-  { admit. }
-  assert (NRMWDOM : ~dom_rel rmw_t' b).
-  { admit. }
-  assert (HEQLAB : lab_t' = lab_t).
-  { admit. }
-  tertium_non_datur (E_t a) as [INA|NINA];
-  tertium_non_datur (E_t b) as [INB|NINB].
-  all: try now (desf; exfalso; eauto).
-  { exists (exec_mapped G_t' mapper (lab_t'  ∘ mapper)),
-           (mapper ↑ sc).
-    replace G_s with (exec_mapped G_t mapper (lab_t ∘ mapper)).
-    { replace lab_t with lab_t' by ins.
-      apply simrel_exec_iff_helper_1; ins.
-      apply SIM. }
-    symmetry. apply exeeqv_eq. apply rsrw_struct_same1; ins.
-    all: try now apply SIM. }
-  assert (U2V : same_label_u2v (lab_s a) (lab_t b)).
-  { rewrite <- ReordCommon.mapper_eq_b with (a := a) (b := b).
-    change (lab_s (mapper b)) with ((lab_s ∘ mapper) b).
-    now apply SIM. }
-  exists (exec_upd_lab
-          (exec_mapped G_t' mapper (lab_t' ∘ mapper))
-        a (lab_s a)), (mapper ↑ sc).
-  replace G_s with (exec_upd_lab
-                      (exec_mapped G_t mapper (lab_t' ∘ mapper))
-                    a (lab_s a)) at 1.
-  { apply simrel_exec_iff_helper_2; ins.
-    { rewrite HEQLAB. now apply same_label_u2v_comm. }
-    apply SIM. }
-  rewrite HEQLAB.
-  symmetry. apply exeeqv_eq. apply rsrw_struct_same2; ins.
-  all: apply SIM.
-Admitted.
-
-Lemma simrel_exec_b_helper sc sw l
-    (U2V : same_label_u2v (lab_t' b) l)
-    (WB_LOC : same_loc (upd (lab_t' ∘ mapper) a l) a sw)
-    (WB_VAL : val (upd (lab_t' ∘ mapper) a l) sw =
-              val (upd (lab_t' ∘ mapper) a l) a)
-    (INA : ~E_t a)
-    (NINB : ~E_t b)
-    (SIM_ACTS : reord_simrel_rw_actids G_t a b)
-    (W_NOT_A : sw <> a)
-    (W_NOT_B : sw <> b)
-    (CONS : WCore.is_cons G_t sc)
-    (STEP : WCore.exec_inst G_t G_t' sc traces a)
-    (HWIN : E_t sw)
-    (W_IS : W_t sw)
-    (NRMWDEP : ~rmw_dep_t' a b)
-    (NRMW : ~rmw_t' a b)
-    (NRMWCODOM : ~codom_rel rmw_t' a)
-    (NRMWDOM : ~dom_rel rmw_t' b) :
-  << STEP1 : WCore.exec_inst
-              (exec_upd_lab
-                (exec_mapped G_t  mapper (lab_t'  ∘ mapper))
-                a l)
-              (exec_add_rf
-                (exec_add_read_event_nctrl
-                  (exec_upd_lab
-                    (exec_mapped G_t mapper (lab_t' ∘ mapper))
-                    a l) a)
-                (singl_rel sw a))
-              (mapper ↑ sc)
-              traces'
-              a >> /\
-  << STEP2 : WCore.exec_inst
-              (exec_add_rf
-                (exec_add_read_event_nctrl
-                  (exec_upd_lab
-                    (exec_mapped G_t mapper (lab_t' ∘ mapper))
-                    a l) a)
-                (singl_rel sw a))
-              (exec_add_rf
-                (exec_add_read_event_nctrl
-                  (exec_upd_lab
-                    (exec_mapped G_t' mapper (lab_t' ∘ mapper))
-                    a l) a)
-                (singl_rel sw a))
-              (mapper ↑ sc)
-              traces'
-              b >>.
-Proof using.
-  assert (B_IS_R : R_t' b).
-  { admit. }
-  assert (W_IS_W' : W_t' sw).
-  { admit. }
-  split.
-  { constructor; ins.
-    { admit. (* Start wf *) }
-    { red. eexists _, _, _, _.
-      splits.
-      { admit. (* TODO: struct *) }
-      { red in U2V.
-        apply cfg_add_event_nctrl_as_add_step; ins.
-        all: unfold compose, is_w, is_r; rupd; ins.
-        { rewrite ReordCommon.mapper_neq; ins. }
-        unfold is_r in B_IS_R. desf. }
-      { admit. (* traces *) }
-      admit. (* End wf -- todo lemma *) }
-    admit. (* IS_cons *) }
-  constructor; ins.
-  { admit. (* Start wf *) }
-  { destruct STEP. red in add_event. desf.
-    exists (option_map mapper r), (option_map mapper w),
-           (mapper ↑₁ W1), (mapper ↑₁ W2).
-    splits.
-    { admit. (* Struct *) }
-    { replace ∅ with (mapper ↑₁ ∅) by now rewrite set_collect_empty.
-      apply cfg_add_event_nctrl_add_step_props with
-        (X := {|
-          WCore.sc := mapper ↑ sc;
-          WCore.G := exec_mapped G_t  _ _;
-          WCore.GC := exec_mapped G_t' _ _;
-          WCore.cmt := mapper ↑₁ ∅
-        |})
-        (X' := {|
-          WCore.sc := mapper ↑ sc;
-          WCore.G := exec_mapped G_t'  _ _;
-          WCore.GC := exec_mapped G_t' _ _;
-          WCore.cmt := mapper ↑₁ ∅
-        |}).
-      { ins. intro F. apply set_collect_empty in F. desf. }
-      apply cfg_upd_lab_add_step_props with
-        (X := {|
-          WCore.sc := mapper ↑ sc;
-          WCore.G := exec_mapped G_t  _ _;
-          WCore.GC := exec_mapped G_t' _ _;
-          WCore.cmt := mapper ↑₁ ∅
-        |})
-        (X' := {|
-          WCore.sc := mapper ↑ sc;
-          WCore.G := exec_mapped G_t'  _ _;
-          WCore.GC := exec_mapped G_t' _ _;
-          WCore.cmt := mapper ↑₁ ∅
-        |}).
-      { ins. unfold compose. now rewrite ReordCommon.mapper_eq_a. }
-      rewrite <- ReordCommon.mapper_eq_a with (a := a) (b := b) at 13.
-      apply cfg_mapped_add_step_props with
-        (X := {|
-            WCore.sc := sc;
-            WCore.G := G_t;
-            WCore.GC := G_t';
-            WCore.cmt := ∅;
-        |})
-        (X' := {|
-            WCore.sc := sc;
-            WCore.G := G_t';
-            WCore.GC := G_t';
-            WCore.cmt := ∅;
-        |}).
-      { apply ReordCommon.mapper_inj. eapply rsrw_a_neq_b; eauto. }
-      { apply ReordCommon.mapper_surj. eapply rsrw_a_neq_b; eauto. }
-      { ins. admit. (* easy easy *) }
-      apply PROPS. }
-    { admit. (* Trace stuff *) }
-    apply WCore.wf_iff_struct_and_props; split.
-    { admit. (* STRUCT *) }
-    replace ∅ with (mapper ↑₁ ∅) by now rewrite set_collect_empty.
-    apply cfg_add_event_nctrl_wf_props with (X := {|
-      WCore.sc := mapper ↑ sc;
-      WCore.G := exec_upd_lab _ a l;
-      WCore.GC := exec_upd_lab _ a l;
-       WCore.cmt := mapper ↑₁ ∅
-    |}); ins.
-    { apply SIM_ACTS. }
-    { admit. (* TODO: condition *) }
-    { admit. (* <-> b is not in E_t', which is true *) }
-    { admit. (* a is a read in source *) }
-    { admit. }
-    { admit. (* WF-ness noise *) }
-    { admit. (* Other wf-ness noise *) }
-    { admit. (* True, because it implies b being in E_t *) }
-    { admit. (* Hyp *) }
-    { basic_solver. }
-    { admit. (* Inferrable from hyps *) }
-    { admit. (* Inferrable from hyps *) }
-    { basic_solver. }
-    { basic_solver. }
-    { admit. }
-    { admit. }
-    apply cfg_upd_lab_wf_props with (X := {|
-      WCore.sc := mapper ↑ sc;
-      WCore.G := exec_mapped _ _ _;
-      WCore.GC := exec_mapped _ _ _;
-      WCore.cmt := mapper ↑₁ ∅;
-    |}); ins.
-    { apply SIM_ACTS. }
-    { unfold compose. now rewrite ReordCommon.mapper_eq_a. }
-    { admit. (* True because b is not in E_t *) }
-    { admit. (* True because b is not in E_t *) }
-    apply cfg_mapped_wf_props with (X := {|
-      WCore.sc := sc;
-      WCore.G := G_t';
-      WCore.GC := G_t';
-      WCore.cmt := ∅;
-    |}); ins.
-    { apply ReordCommon.mapper_inj. eapply rsrw_a_neq_b; eauto. }
-    { apply ReordCommon.mapper_surj. eapply rsrw_a_neq_b; eauto. }
-    { admit. (* TODO: easy *) }
-    { apply ReordCommon.mapper_init_actid.
-      all: apply SIM_ACTS. }
-    { apply ReordCommon.mapped_G_t_immsb_helper.
-      all: admit. }
-    { apply ReordCommon.mapped_G_t_sb_helper.
-      all: admit. }
-    { admit. (* TODO *) }
-    { admit. (* WFness noise *) }
-    { apply start_wf. }
-    { apply start_wf. }
-    { apply start_wf. }
-    apply WF_NEW. }
-  admit. (* IS_cons *)
-Admitted.
-
-Lemma simrel_exec_b sc
-    (CONS : WCore.is_cons G_t sc)
-    (CONS' : WCore.is_cons G_s (mapper ↑ sc))
-    (SIM : reord_simrel_rw G_s G_t a b)
     (STEP : WCore.exec_inst G_t G_t' sc traces a) :
-  exists G_s' sc',
-    << SIM' : reord_simrel_rw G_s' G_t' a b >> /\
-    exists G_s'_int,
-      << STEP1 : WCore.exec_inst G_s G_s'_int sc' traces' a >> /\
-      << STEP2 : WCore.exec_inst G_s'_int G_s' sc' traces' b >>.
-Proof using SWAPPED_TRACES.
-  admit. (* TODO: research *)
-Admitted.
-
-Lemma simrel_exec_a_helper sc w sw l
-    (CONS : WCore.is_cons G_t sc)
-    (CONS' : WCore.is_cons G_s (mapper ↑ sc))
-    (RF : rf_t' w b)
-    (SIM_ACTS : reord_simrel_rw_actids G_t a b)
-    (STEP : WCore.exec_inst G_t G_t' sc traces b) :
-  exists dtrmt cmt,
-    WCore.reexec
-      (exec_add_rf
-        (exec_add_read_event_nctrl
-          (exec_upd_lab
-            (exec_mapped G_t mapper (lab_t' ∘ mapper))
-            a l) a)
-        (singl_rel sw a))
-      (exec_mapped G_t' mapper (lab_t'  ∘ mapper))
-      (mapper ↑ sc)
-      traces'
-      dtrmt
-      cmt.
-Proof using.
-  (* Shorthands *)
-  set (G_s_ := exec_add_rf
-    (exec_add_read_event_nctrl
-      (exec_upd_lab
-        (exec_mapped G_t mapper (lab_t' ∘ mapper))
-        a l) a)
-    (singl_rel sw a)).
-  set (G_s' :=
-    exec_mapped G_t' mapper (lab_t'  ∘ mapper)).
-  set (dtrmt := mapper ↑₁ E_t \₁ codom_rel (
-    ⦗eq a⦘ ⨾ (sb G_s_ ∪ rf G_s_)＊
-  )).
-  set (delta := acts_set G_s' \₁ dtrmt).
-  set (cmt := acts_set G_s_ \₁ eq a).
-  set (f := fun x => ifP cmt x then Some x else None).
-  (* Asserts *)
-  assert (DTRMT_INIT : mapper ↑₁ E_t' ∩₁ is_init ⊆₁ dtrmt).
+  exists G_s' sc' G_s'',
+    << SIMREL : reord_simrel_rw G_s' G_t' a b >> /\
+    << STEP1 : WCore.exec_inst G_s   G_s'' sc' traces' a >> /\
+    << STEP2 : WCore.exec_inst G_s'' G_s'  sc' traces' b >>.
+Proof using SIMREL.
+  (* Preamble *)
+  destruct STEP as [STARTWF ADD]. red in ADD. desf.
+  destruct (classic (E_t a)) as [INA|NINA].
+  { exfalso. now apply (WCore.caes_e_notin STRUCT). }
+  destruct (classic (E_t b)) as [INB|NINB].
+  { exfalso. eapply rsrw_actids_t_ord; eauto.
+    apply SIMREL. }
+  assert (CASE2KILLER : ~~(E_t' a /\ ~E_t' b)).
   { admit. }
-  assert (ACTEQ : E_t' ≡₁ E_t ∪₁ eq b).
-  { admit. (* TODO: use step *) }
-  assert (WINE : E_t w).
+  destruct srf_eq as (sw & SRFEQ); eauto.
   { admit. }
   (* Actual proof *)
-  admit.
+  exists G_s', (mapper ↑ sc), (rsrw_G_s_niff G_s G_t a b).
+  unfold NW. rewrite G_s_iff at 1; ins.
+  unfold G_s'. desf.
+  splits; constructor; ins.
+  { admit. (* TODO: simrel actids *) }
+  { admit. (* TODO: simrel struct *) }
+  { admit. (* TODO: step1 start wf *) }
+  { exists None, (Some sw), ∅, ∅.
+    splits.
+    { admit. (* TODO: STRUCT *) }
+    { admit. (* TODO: cfg_add_event_nctrl_as_add_step *) }
+    { admit. (* TODO: traces *) }
+    admit. (* TODO: result wf *) }
+  { admit. (* TODO: intermediate cons *) }
+  { admit. (* TODO: wf of finish *) }
+  { desf.
+    exists (option_map mapper r), (option_map mapper w),
+           (mapper ↑₁ W1), (mapper ↑₁ W2).
+    splits.
+    { constructor; ins.
+      { rewrite (WCore.caes_e_new STRUCT), set_collect_union. ins.
+        rewrite set_collect_eq, ReordCommon.mapper_eq_a.
+        basic_solver 12. }
+      { admit. (* TODO: easy *) }
+      apply SIMREL. }
+    { rewrite rsrw_X_s'_niff_eq, rsrw_X_s_niff_eq; ins.
+      replace b with (mapper a) at 1 by now rewrite ReordCommon.mapper_eq_a.
+      unfold rsrw_X_s_niff, rsrw_X_s'_niff.
+      rewrite SRFEQ.
+      apply cfg_add_event_nctrl_add_step_props.
+      { ins. admit. }
+      apply cfg_upd_lab_add_step_props.
+      { ins. admit. }
+      eapply cfg_mapped_add_step_props; ins.
+      all: admit. }
+    { admit. (* TODO: traces *) }
+    admit. (* TODO WF *) }
+  admit. (* TODO: cons of finish *)
 Admitted.
 
-Lemma simrel_exec_a sc w
-    (CONS : WCore.is_cons G_t sc)
-    (CONS' : WCore.is_cons G_s (mapper ↑ sc))
+Lemma simrel_exec_a w
     (RF : rf_t' w a)
-    (SIM : reord_simrel_rw G_s G_t a b)
+    (CONS : WCore.is_cons G_t sc)
     (STEP : WCore.exec_inst G_t G_t' sc traces b) :
   exists G_s' sc' dtrmt' cmt',
-    << SIM' : reord_simrel_rw G_s' G_t' a b >> /\
+    << SIM : reord_simrel_rw G_s' G_t' a b >> /\
     << STEP : WCore.reexec G_s G_s' sc' traces' dtrmt' cmt' >>.
-Proof using SWAPPED_TRACES.
-  (* TODO: check article *)
-  (* Case1 : Gt' *)
-  (* Case2: mapped Gt but with executed a *)
+Proof using SIMREL.
   admit.
 Admitted.
 
